Test/civl/async/lock-service.bpl
@@ -1,7 +1,7 @@
 // RUN: %parallel-boogie "%s" > "%t"
 // RUN: %diff "%s.expect" "%t"
 
-type {:linear "tid"} Tid = int;
+type Tid = int;
 
 const nil:Tid;
 var {:layer 0,4} l:Tid;
@@ -12,28 +12,28 @@ modifies x;
 {
   x := x + 1;
 }
-yield procedure {:layer 4} Client({:hide}{:linear_in "tid"} tid:Tid)
+yield procedure {:layer 4} Client({:hide}{:linear_in} tid: One Tid)
 refines A_Client;
-requires {:layer 4} tid != nil;
+requires {:layer 4} tid->val != nil;
 {
   call GetLockAndCallback(tid);
 }
 
-atomic action {:layer 4} A_GetLockAndCallback' ({:linear_in "tid"} tid:Tid)
+atomic action {:layer 4} A_GetLockAndCallback' ({:linear_in} tid: One Tid)
 modifies x;
 {
-  assert tid != nil;
+  assert tid->val != nil;
   x := x + 1;
 }
 
-async left action {:layer 3} A_Callback ({:linear_in "tid"} tid:Tid)
+async left action {:layer 3} A_Callback ({:linear_in} tid: One Tid)
 modifies l, x;
 {
-  assert tid != nil && l == tid;
+  assert tid->val != nil && l == tid->val;
   x := x + 1;
   l := nil;
 }
-yield procedure {:layer 2} Callback ({:linear_in "tid"} tid:Tid)
+yield procedure {:layer 2} Callback ({:linear_in} tid: One Tid)
 refines A_Callback;
 {
   var tmp:int;
@@ -42,16 +42,16 @@ refines A_Callback;
   async call {:sync} ReleaseLock(tid);
 }
 
-both action {:layer 2} A_read_x_lock ({:linear "tid"} tid:Tid) returns (v:int)
-{ assert tid != nil && l == tid; v := x; }
-yield procedure {:layer 1} read_x_lock ({:linear "tid"} tid:Tid) returns (v:int)
+both action {:layer 2} A_read_x_lock ({:linear} tid: One Tid) returns (v:int)
+{ assert tid->val != nil && l == tid->val; v := x; }
+yield procedure {:layer 1} read_x_lock ({:linear} tid: One Tid) returns (v:int)
 refines A_read_x_lock;
 { call v := read_x(); }
 
-both action {:layer 2} A_write_x_lock (v:int, {:linear "tid"} tid:Tid)
+both action {:layer 2} A_write_x_lock (v:int, {:linear} tid: One Tid)
 modifies x;
-{ assert tid != nil && l == tid; x := v; }
-yield procedure {:layer 1} write_x_lock (v:int, {:linear "tid"} tid:Tid)
+{ assert tid->val != nil && l == tid->val; x := v; }
+yield procedure {:layer 1} write_x_lock (v:int, {:linear} tid: One Tid)
 refines A_write_x_lock;
 { call write_x(v); }
 
@@ -69,51 +69,51 @@ refines A_write_x;
 // -----------------------------------------------------------------------------
 
 atomic action {:layer 3}
-A_GetLockAndCallback ({:linear_in "tid"} tid:Tid)
+A_GetLockAndCallback ({:linear_in} tid: One Tid)
 refines A_GetLockAndCallback';
 creates A_Callback;
 modifies l;
 {
-  assert tid != nil;
+  assert tid->val != nil;
   assume l == nil;
-  l := tid;
+  l := tid->val;
   call create_async(A_Callback(tid));
 }
-yield procedure {:layer 2} GetLockAndCallback ({:linear_in "tid"} tid:Tid)
+yield procedure {:layer 2} GetLockAndCallback ({:linear_in} tid: One Tid)
 refines A_GetLockAndCallback;
 {
   call GetLock(tid);
   async call Callback(tid);
 }
 
-atomic action {:layer 2} A_GetLock ({:linear "tid"} tid:Tid)
+atomic action {:layer 2} A_GetLock ({:linear} tid: One Tid)
 modifies l;
 {
-  assert tid != nil;
+  assert tid->val != nil;
   assume l == nil;
-  l := tid;
+  l := tid->val;
 }
-yield procedure {:layer 1} GetLock ({:linear "tid"} tid:Tid)
+yield procedure {:layer 1} GetLock ({:linear} tid: One Tid)
 refines A_GetLock;
 {
   var success:bool;
   while (true)
   invariant {:yields} true;
   {
-    call success := cas_l(nil, tid);
+    call success := cas_l(nil, tid->val);
     if (success) {
       return;
     }
   }
 }
 
-left action {:layer 2} A_ReleaseLock ({:linear_in "tid"} tid:Tid)
+left action {:layer 2} A_ReleaseLock ({:linear_in} tid: One Tid)
 modifies l;
 {
-  assert tid != nil && l == tid;
+  assert tid->val != nil && l == tid->val;
   l := nil;
 }
-yield procedure {:layer 1} ReleaseLock ({:linear_in "tid"} tid:Tid)
+yield procedure {:layer 1} ReleaseLock ({:linear_in} tid: One Tid)
 refines A_ReleaseLock;
 {
   call write_l(nil);
